iris/SpecKexecB3.v
@@ -91,7 +91,7 @@ Definition kxc_b2_body
  (pd pav pu : mword 64)
     (gilf gislf : gname) (gf : gname)
     (kf : nat) (qf sf : Qp) (gyf : gname) (loyf tlyf : nat) (inumf : mword 32)
-    (dnf : dinode) (bmf : blkmap) (n2 : nat)
+    (dnf : dinode) (bmf : blkmap) (datl : nat -> list (bv 8)) (n2 : nat)
     (plen : nat) (pfun : nat -> bv 8)
     (na : nat) (avf : nat -> mword 64) (alen aslen : nat -> nat)
     (afun : nat -> nat -> bv 8)
@@ -120,7 +120,7 @@ Definition kxc_b2_body
   fs_fabric gs pd pav pu
  -∗
   kxc_at_12c jp gf
- kf qf sf gyf loyf tlyf inumf dnf bmf gilf gislf n2
+ kf qf sf gyf loyf tlyf inumf dnf bmf datl gilf gislf n2
              plen pfun na avf aslen afun pidv U eb dqb dqs dqa dqpv dqas m M K
              sp0 ra0 s00 s10 s20 pv av
              (m !!! Regidx Rs3) (m !!! Regidx Rs4) (m !!! Regidx Rs5)
@@ -157,7 +157,7 @@ Definition kxc_b2z_body
  (pd pav pu : mword 64)
     (gilf gislf : gname) (gf : gname)
     (kf : nat) (qf sf : Qp) (gyf : gname) (loyf tlyf : nat) (inumf : mword 32)
-    (dnf : dinode) (bmf : blkmap) (n2 : nat)
+    (dnf : dinode) (bmf : blkmap) (datl : nat -> list (bv 8)) (n2 : nat)
     (plen : nat) (pfun : nat -> bv 8)
     (na : nat) (avf : nat -> mword 64) (alen aslen : nat -> nat)
     (afun : nat -> nat -> bv 8)
@@ -181,7 +181,7 @@ Definition kxc_b2z_body
   fs_fabric gs pd pav pu
  -∗
   kxc_at_1a2 jp gf
- kf qf sf gyf loyf tlyf inumf dnf bmf gilf gislf n2
+ kf qf sf gyf loyf tlyf inumf dnf bmf datl gilf gislf n2
              plen pfun na avf aslen afun pidv U eb dqb dqs dqa dqpv dqas m M K
              sp0 ra0 s00 s10 s20 pv av
              (m !!! Regidx Rs3) (m !!! Regidx Rs4) (m !!! Regidx Rs5)
@@ -208,7 +208,7 @@ Module Type KEXECB3.
  (pd pav pu : mword 64)
       (gilf gislf : gname) (gf : gname)
       (kf : nat) (qf sf : Qp) (gyf : gname) (loyf tlyf : nat) (inumf : mword 32)
-      (dnf : dinode) (bmf : blkmap) (n2 : nat)
+      (dnf : dinode) (bmf : blkmap) (datl : nat -> list (bv 8)) (n2 : nat)
       (plen : nat) (pfun : nat -> bv 8)
       (na : nat) (avf : nat -> mword 64) (alen aslen : nat -> nat)
       (afun : nat -> nat -> bv 8)
@@ -218,7 +218,7 @@ Module Type KEXECB3.
       (ef : nat -> bv 8) (P : uptd) (Mi : gmap Z (bv 8)) (i : nat) (szv : mword 64),
     kxc_b2_body Q gs jp gl pd pav pu gilf gislf
  gf
-      kf qf sf gyf loyf tlyf inumf dnf bmf n2 plen pfun na avf alen aslen afun
+      kf qf sf gyf loyf tlyf inumf dnf bmf datl n2 plen pfun na avf alen aslen afun
       pidv U eb dqb dqs dqa dqpv dqas m M K sp0 ra0 s00 s10 s20 pv av w67
       ef P Mi i szv.
 
@@ -228,7 +228,7 @@ Module Type KEXECB3.
  (pd pav pu : mword 64)
       (gilf gislf : gname) (gf : gname)
       (kf : nat) (qf sf : Qp) (gyf : gname) (loyf tlyf : nat) (inumf : mword 32)
-      (dnf : dinode) (bmf : blkmap) (n2 : nat)
+      (dnf : dinode) (bmf : blkmap) (datl : nat -> list (bv 8)) (n2 : nat)
       (plen : nat) (pfun : nat -> bv 8)
       (na : nat) (avf : nat -> mword 64) (alen aslen : nat -> nat)
       (afun : nat -> nat -> bv 8)
@@ -238,6 +238,6 @@ Module Type KEXECB3.
       (ef : nat -> bv 8) (P : uptd) (Mi : gmap Z (bv 8)),
     kxc_b2z_body gs jp gl pd pav pu gilf gislf
  gf
-      kf qf sf gyf loyf tlyf inumf dnf bmf n2 plen pfun na avf alen aslen afun
+      kf qf sf gyf loyf tlyf inumf dnf bmf datl n2 plen pfun na avf alen aslen afun
       pidv U eb dqb dqs dqa dqpv dqas m M K sp0 ra0 s00 s10 s20 pv av w13 w67 ef P Mi.
 End KEXECB3.
